\documentclass[12pt]{article}

\topmargin -40pt
\marginparwidth 0pt
 \oddsidemargin  -40pt
 \evensidemargin 0pt
 \marginparsep 0pt
\textwidth 7.2 in
 \textheight  10 in
 \hoffset  0.1in
\linespread{1.9}

\usepackage{amsthm,amsmath,amssymb,amscd,verbatim,epsfig}
\usepackage{mathptmx}
\usepackage{amsfonts}
%\usepackage{setapace}
\usepackage{graphicx}
\usepackage{bm}
%\usepackage{CJK}
\usepackage{ulem}
\usepackage{multicol}
\usepackage{enumerate}
\usepackage{float}
\usepackage{fontspec}
\usepackage{xeCJK}
\setmainfont{Times New Roman}
\setCJKmainfont{TaipeiSansTCBeta-Regular}
\XeTeXlinebreaklocale "zh"
\XeTeXlinebreakskip = 0pt plus 1pt

\title{Homework 8 of Introduction to Analysis(II)}
\author{AM15 黃琦翔 111652028}

\begin{document}
\maketitle
\begin{enumerate}
    \item $f_x(0, 0) = \displaystyle\lim_{x\to 0} \dfrac{f(x, 0) - f(0)}{x} = \displaystyle\lim_{x\to 0} \dfrac{x\cdot 0(x^2-0^2)/(x^2+0^2)}{x} = 0$ exists.
    Also, we can esaily get that $f_y(0, 0) = 0$.
    Then, $f_{xy}(0, 0) = \dfrac{\partial f_x}{\partial y}(0, 0) = \displaystyle\lim_{y\to 0} \dfrac{y(0^4+4\cdot 0^2y^2 - y^4)/(0^2 + y^2)^2}{y} = \displaystyle\lim_{y\to 0} \dfrac{-y^4}{y^4} = -1$.
    And, $f_{yx}(0, 0) = 1$.
    Therefore, $f_{xy}(0, 0) \neq f_{y}(0, 0)$.

    \item Since $Df$ is continuous on $S$, for any $\epsilon > 0$, there exists $\delta > 0$ s.t. $\| f(x) - f(y)\| < \dfrac{\epsilon}{\|b-a\|}$ if $\| x - y\| < \delta$.
    And since $S$ is a closed line in $R^p$, we can find a sequence $\{ x_k\}_{k=1}^n$ s.t. $D(x_k, \dfrac{\delta}{2}) \supseteq S$ and $\|x_k+1 - a\| > \| x_k - a\|$.
    Let $x_0 = a$ and $x_{n+1} = b$.
    Then, by MCT, $Df(x_1) - Df(a) = Df(c_1)(x_1 - a)$ for $c_1$ on the line between $a, x_1$ and $c_k$ on the line between $x_k, x_k-1$.

    Thus, 
    \begin{align*}
        |f(b) - f(a) - \int_{0}^{1} Df(tb + (1-t)a)(b - a)\ dt| &\leq \sum_{k=1}^{n+1} \|f(x_k) - f(x_{k-1}) - \int_{0}^{1} Df(tx_k + (1-t)x_{k-1})(b-a) dt\|\\
        &= \sum_{k=1}^{n+1} \| \int_{0}^{1} Df(c_k)(x_k - x_{k-1})\ dt\\
        &- \int_{0}^{1} Df(tx_k + (1-t)x_{k-1})(b-a)\ dt\|\\
        &< \dfrac{\epsilon}{b-a} (b-a)\\
        &= \epsilon
    \end{align*}

    Therefore, $f(b) = f(a) = \int_{0}^{1} Df(tb + (1-t)a)(b-a)\ dt$.

    \item $\displaystyle\lim_{u\to x}\|g(u) - g(x) - Dg(x)(u)\|$    
\end{enumerate}
\end{document} 