\documentclass[12pt]{article}

\topmargin -40pt
\marginparwidth 0pt
 \oddsidemargin  -40pt
 \evensidemargin 0pt
 \marginparsep 0pt
\textwidth 7.2 in
 \textheight  10 in
 \hoffset  0.1in
\linespread{1.9}

\usepackage{amsthm,amsmath,amssymb,amscd,verbatim,epsfig}
\usepackage{mathptmx}
\usepackage{amsfonts}
%\usepackage{setapace}
\usepackage{graphicx}
\usepackage{bm}
%\usepackage{CJK}
\usepackage{ulem}
\usepackage{multicol}
\usepackage{enumerate}
\usepackage{float}
\usepackage{fontspec}
\usepackage{xeCJK}
\setmainfont{Times New Roman}
\setCJKmainfont{TaipeiSansTCBeta-Regular}
\XeTeXlinebreaklocale "zh"
\XeTeXlinebreakskip = 0pt plus 1pt

\DeclareMathOperator{\volume}{Vol}
\DeclareMathOperator{\interior}{int}
\DeclareMathOperator{\closure}{cl}
\newcommand{\boundary}{\partial}

\title{Homework 12 of Introduction to Analysis(II)}
\author{AM15 黃琦翔 111652028}

\begin{document}
\maketitle
\begin{enumerate}
    \item \begin{enumerate}
        \item Since  $\boundary \interior(E) = \closure(\interior(E)) \setminus \interior(\interior(E)) = \closure(E) \setminus \interior(E) = \boundary E$ and $\boundary \closure(E) = \boundary E$,
        we can get $\volume(\boundary\interior(E)) = \volume(\boundary\closure(E)) = \volume(\boundary E) = 0$ and $\interior(E), \closure(E)$ are Jordan regions.

        \item Since $\closure(E) = \interior(E) \cup \boundary E$ and $\interior(E)\subseteq E \subseteq \closure(E)$,

        $\volume(\closure(E)) \leq \volume(\interior(E)) + \volume(\boundary E) = \volume(\interior(E))\leq \volume(E) \leq \volume(\closure(E))$.

        Therefore, $\volume(\closure(E)) = \volume(\interior(E)) = E$.

        \item $\ $
        \begin{enumerate}
            \item[$(\implies)$] From $(b)$, we know $\volume(\interior(E)) = \volume(E) > 0$, 
            then for any $\epsilon > 0$, we can find a set of rectangles $R_n$ s.t. $\volume(E) > \sum |R_n| > \volume(E) - \epsilon$ and $\cup R_n \subseteq \interior(E)$.
            Therefore, $\interior(E) \neq \emptyset$.

            \item[$(\impliedby)$] Since $\interior(E)$ is non-empty, for any $x_0\in \interior(E)$, there exists $\epsilon > 0$ s.t. $D(x_0, \epsilon) \subseteq \interior(E)$.
            Then, we can find a small rectangle $R$ with each length is $\dfrac{\epsilon}{n}$ and $R$ is contained in $D(x_0, \epsilon)$.
            Thus, $\volume(\interior(E)) > \left(\dfrac{\epsilon}{n}\right)^n > 0$.
        \end{enumerate}

        \item Since $f$ is continuous, for any $x_0 \in [a, b]$, we can find a sequence $x_k \to x_0$ s.t. $f(x_k) \to f(x_0)$.
        That is, $A = \{(x, f(x)) \mid x\in [a, b]\}$ is closed.
        And since $\boundary A \subseteq A$, $\volume(\boundary A) \leq \volume(A)$.
        
        Since $f$ is continuous on $[a, b]$ is compact, for all $\epsilon > 0$, we can find $\delta > 0$ s.t. $|x-y| < \delta$ implies That $|f(x) - f(y)| < \dfrac{\epsilon}{b-a}$.
        Then, we can find a finite increasing sequence $\{x_i \mid x_i \in [a, b]\}_{i=1}^N$ s.t. $[a, b] \subseteq D(x_i, \dfrac{\delta}{2})$.
        Therefore, for any $y = f(x)$, $y \in D(f(x_i), \dfrac{\epsilon}{b-a})$ for some $i$.

        Then, take $u_0 = a$, $u_i \in D(x_i, \dfrac{\delta}{2})\cap D(x_{i+1}, \dfrac{\delta}{2})$, $u_N = b$,
        and we can get $[a, b] = \cup [u_i, u_{i+1}]$.
        Thus, $A \subseteq \displaystyle\bigcup_{i=0}^N [u_i, u_{i+1}] \times D(\xi_i, \dfrac{\epsilon}{b-a})$ for some $\xi_i \in \{ f(x)\mid x\in [u_i, u_{i+1}]\}$
        with the sum of the rectangles is $2\dfrac{\epsilon}{b-a} \cdot (b-a) = 2\epsilon$.
        Hence, $\volume(A) = 0$ and $\volume(\boundary A) = 0$.

        \item Yes. Since $f$ is integrable, for any $\epsilon > 0$, 
        we can find an partition $P$ s.t. $|U(f, P) - L(f, P)|< \epsilon$.
        That is, $\displaystyle\sum_{i=0}^{N} (\displaystyle\sup_{x\in [x_i, x_{i+1}]}\{f(x)\} - \displaystyle\inf_{x\in [x_i, x_{i+1}]}\{f(x)\}) \cdot (x_{i+1} - x_i) < \epsilon$,
        and each one of the summation is a rectangle that contains all $(x, f(x))$ in the intevral.
        Thus, $\volume(A) = 0$ and $\volume(\boundary A) = 0$.
    \end{enumerate}

    \item \begin{enumerate}
        \item $\boundary (E_1 \cap E_2) = \closure(E_1 \cap E_2) \cap \closure(M\setminus E_1 \cap E_2) \subseteq (\closure(E_1) \cap \closure(M \setminus E_1)) \cup (\closure(E_2) \cap \closure(M\setminus E_2)) = \boundary E_1 \cup \boundary E_2$.
        Then, $\volume(\boundary (E_1 \cap E_2)) \leq \volume(\boundary E_1) + \volume(\boundary E_2) = 0$.
        
        Also $\boundary (E_1 \setminus E_2) \subseteq \boundary E_1 \cup \boundary E_2$.
        Therefore, $E_1 \cap E_2$ and $E_1 \setminus E_2$ are Jordan regions.
    
        \item Since $E_1, E_2$ are non-overlapping, $E_1 \cap E_2 \subseteq \boundary E_1 \cup \boundary E_2$.
        And since $E_1, E_2$ are Jordan regions, $\volume(E_1) = \volume(\interior(E_1))$ and $\volume(E_2) = \volume(\interior(E_2))$.
        Also we have $\interior(E_1) \cup \interior(E_2) \subseteq E_1 \cup E_2$ and $\interior(E_1) \cap \interior(E_2) = \emptyset$.

        \begin{align*}
            \volume(\interior(E_1)) + \volume(\interior(E_1)) &= \volume(\interior(E_1) \cup \interior(E_2))\\
            &\leq \volume(\interior(E_1) \cup \interior(E_2)) + \volume(E_1 \cap E_2)\\
            &= \volume(E_1 \cup E_2)\\
            &\leq \volume(\interior(E_1)) + \volume(\interior(E_1)) + \volume(\boundary E_1) + \volume(\boundary E_2)\\
            &= \volume(\interior(E_1)) + \volume(\interior(E_2))\\
            &= \volume(E_1) + \volume(E_2)
        \end{align*}
        Thus, $\volume(E_1\cup E_2) = \volume(E_1) + \volume(E_2)$.

        \item Let $E_1\setminus E_1 = S_1$, $E_2 = S_2$.
        We have $S_1$ and $S_2$ are Jordan regions and non-overlapping.
        Thus, $\volume(E_1) = \volume(S_1 \cup S_2) = \volume(S_1) + \volume(S_1)$ and 
        $\volume(E_1\setminus E_2) = \volume(E_1) - \volume(E_2)$.

        \item Using (b), (c) and the fact $E_1 \cup E_2 = (E_1 \setminus E_1 \cap E_2) \cup (E_1 \cap E_2) \cup (E_2 \setminus E_2\cap E_1)$,
        we can get $\volume(E_1 \cup E_2) = (\volume(E_1) - \volume(E_1 \cap E_2)) + \volume(E_1 \cap E_2) + (\volume(E_2) - \volume(E_1 \cap E_2)) = \volume(E_1) + \volume(E_2) - \volume(E_1\cap E_2)$.
    \end{enumerate}
\end{enumerate}
\end{document} 