\documentclass[12pt]{article}

\topmargin -40pt
\marginparwidth 0pt
 \oddsidemargin  -40pt
 \evensidemargin 0pt
 \marginparsep 0pt
\textwidth 7.2 in
 \textheight  10 in
 \hoffset  0.1in
\linespread{1.9}

\usepackage{amsthm,amsmath,amssymb,amscd,verbatim,epsfig}
\usepackage{mathptmx}
\usepackage{amsfonts}
%\usepackage{setapace}
\usepackage{graphicx}
\usepackage{bm}
%\usepackage{CJK}
\usepackage{ulem}
\usepackage{multicol}
\usepackage{enumerate}
\usepackage{float}
\usepackage{fontspec}
\usepackage{xeCJK}
\setmainfont{Times New Roman}
\setCJKmainfont{TaipeiSansTCBeta-Regular}
\XeTeXlinebreaklocale "zh"
\XeTeXlinebreakskip = 0pt plus 1pt

\title{Homework 2 of Introduction to Analysis(II)}
\author{AM15 黃琦翔 111652028}

\begin{document}
\maketitle
\begin{enumerate}
    \item For all $\epsilon > 0$, we can find a $N \in \mathbb{N}$ s.t. $|a_n - a| < \dfrac{\epsilon}{2}$ for all $n > N$.
    And we can find a $N' > N$ s.t. $\dfrac{\displaystyle\sum_{i=1}^{N} a_i - a}{N'} < \dfrac{\epsilon}{2}$.
    Thus, for any $n > N'$, \begin{align*}
        |\dfrac{\sum_{i=1}^{n} a_i }{n} - a| &\leq |\dfrac{\sum_{i=1}^{N} a_i - a}{n}| + |\dfrac{\sum_{i=N+1}^{n} a_i - a}{n - N'}|\\
        &< \dfrac{\epsilon}{2} + \dfrac{\epsilon}{2}\\
        &= \epsilon
    \end{align*}
    Therefore, $\displaystyle\lim_{n\to\infty} b_n = a$.

    \item Since $\displaystyle\lim_{n\to\infty} na_n = 0$, by 1., $\displaystyle\lim_{N\to\infty} \displaystyle\sum_{n=0}^{N} a_n = \displaystyle\lim_{N\to\infty} \displaystyle\sum_{n=0}^{N} \dfrac{na_n}{N} = 0$
    Also, since $\displaystyle\lim_{n\to\infty} na_n = 0$, $\displaystyle\lim_{n\to\infty} a_n = 0$.

    Thus, for any $\epsilon > 0$,  there exists a $N \in \mathbb{N}$ s.t. $|\displaystyle\sum_{n=0}^{k} a_n| < \dfrac{\epsilon}{2}$ for all $k > N$.
    
    Then, for $x \to 1^{-}$ s.t. $|f(x) - A| < \dfrac{\epsilon}{2}$, \begin{align*}
        \sum_{n=0}^{N} a_n - A &= \sum_{n=0}^{N} a_n(1-x^n) - \sum_{n=N+1}^{\infty} a_n x^n + (f(x) - A)\\
        &\leq \dfrac{\epsilon}{2} - 0 + \dfrac{\epsilon}{2}\\
        &= \epsilon
    \end{align*}
    
    Therefore, $\displaystyle\sum_{n=0}^{\infty} a_n = A$.

    \item 
\end{enumerate}
\end{document}